MPL/Experimental/Crush.lean
@@ -1,0 +1,41 @@
+/-
+Copyright (c) 2025 Lean FRO LLC. All rights reserved.
+Released under Apache 2.0 license as described in the file LICENSE.
+Authors: Sebastian Graf
+-/
+import Lean
+import MPL.Triple
+import MPL.SpecAttr
+
+import MPL.Specs
+import MPL.WPMonad
+import MPL.WPMonadLift
+import MPL.WPMonadFunctor
+import MPL.WPMonadExceptOf
+import MPL.WPSimp
+import MPL.SPred.ProofMode
+
+namespace MPL
+
+open Lean Meta Elab Tactic
+
+syntax "crush_trivial" : tactic
+macro_rules | `(tactic| crush_trivial) => `(tactic| trivial)
+
+syntax (name := crush) "crush" optional("[" Lean.Parser.Tactic.simpLemma,+ "]") : tactic
+macro_rules
+  | `(tactic| crush) => `(tactic| crush[if_true_left]) -- if_true_left is redundant, but empty list did not work for some reason.
+  | `(tactic| crush [$args,*]) => `(tactic| (intros; first
+    | (intro; repeat intro) -- expand ≤ on → and Assertions, also turns triple goals into wp goals
+    | crush_trivial
+    | simp_all only [if_true_left, if_false_left, and_self, and_true, List.length_nil, List.length_cons, ne_eq, not_false_eq_true, gt_iff_lt
+        , reduceIte
+        , Nat.sub_one_add_one
+        , SVal.curry_nil
+        , PostCond.total
+      ]
+    | (simp_all [$args,*, Nat.sub_one_add_one]; done)
+    -- | grind
+    ))
+
+end MPL
