Test/Demo.lean
@@ -182,7 +182,7 @@ theorem fib_triple : ⦃True⦄ fib_impl n ⦃⇓ r => r = fib_spec n⦄ := by
   simp only [h, reduceIte]
   mspec Specs.forIn_list ?inv ?step
   case inv => exact PostCond.total fun (⟨a, b⟩, xs) => a = fib_spec xs.rpref.length ∧ b = fib_spec (xs.rpref.length + 1)
-  case pre => simp_all
+  case pre1 => simp_all
   case step => intros; mintro _; mwp; simp_all
   simp_all [Nat.sub_one_add_one]
 
